examples/CCS/Denotation.v
@@ -237,6 +237,13 @@ Proof.
     rewrite <- eq1; eauto.
 Qed.
 
+Lemma trans_brS' {E C X Y} : forall (c : C Y) (k : Y -> ctree E C X) x u,
+    u ≅ k x ->
+		trans τ (BrS c k) u.
+Proof.
+  intros * eq; rewrite eq; apply trans_brS.
+Qed.
+
 Lemma trans_prefix_inv : forall l a p p',
     trans l (prefix a p) p' ->
     p' ≅ p /\ l = comm a.
@@ -268,27 +275,6 @@ Lemma trans_vis' {E C R X} : forall (e : E X) x (k : X -> ctree E C R) u,
     trans (obs e x) (Vis e k) u.
 Proof.
   intros * eq; rewrite eq; apply trans_vis.
-Qed.
-
-(** ** prefix *)
-
-Ltac inv_ccs_trans :=
-  match goal with
-  | h : hrel_of (trans _) (prefix _ _) _ |- _ => apply trans_prefix_inv in h as (?EQ & ->)
-  | _ => idtac
-  end.
-Hint Resolve trans_prefix : ccs.
-Ltac ccs_trans := eauto with ccs.
-
-#[global] Instance prefix_st a: forall (R : Chain (sb eq)),
-    Proper (elem R ==> elem R) (prefix a).
-Proof.
-  apply (Proper_symchain 1).
-  intros R HR p q Hpq l p' pp'.
-  inv_ccs_trans.
-  eex; ssplit; ccs_trans.
-  rewrite EQ.
-  now step.
 Qed.
 
 (** ** hnew *)
@@ -387,23 +373,14 @@ Proof.
   - tauto.
 Qed.
 
-Lemma trans_new_inv : forall l c p p',
-    trans l (new c p) p' ->
-    exists q, can_comm c l = true /\ trans l p q /\ p' ≅ Guard (new c q).
-Proof.
-  intros.
-  unfold new in H.
-  eapply trans_new_inv_aux. eapply H.
-  all: rewrite <- ctree_eta; auto.
-Qed.
-
-
 Lemma trans_new_inv_aux : forall l T U,
     trans_ l T U ->
     forall c p q,
       (go T ≅ new c p \/ go T ≅ Guard (new c p)) ->
       go U ≅ q ->
-      exists q', can_comm c l = true /\ trans l p q' /\ q ≅ Guard (new c q').
+      exists q', can_comm c l = true /\ trans l p q' /\
+            q ≅ Guard (new c q').
+            (* /\ (q ≅ Guard (new c q') \/ q ≅ new c q'). *)
 Proof.
   intros * tr c.
   induction tr; intros * EQ1 EQ2; try destruct c2.
@@ -441,80 +418,70 @@ Proof.
       cbn.
       desobs p; try now (step in EQ1; inv EQ1).
       * inv_equ.
-
-        edestruct (IHtr t) as (q' & comm & tr' & EQ).
-        right; rewrite <- ctree_eta, EQ1.
-        now left; rewrite <- ctree_eta.
-        eauto.
-        exists q'; repeat split; auto.
-        eapply trans_br with (x := x).
-        eauto.
+        edestruct (IHtr t0) as (q' & comm & tr' & EQ).
+        left. rewrite EQ1. rewrite <- ctree_eta.
         reflexivity.
-
-        eauto.
-
-
-        destruct e,a; cbn in *.
-        ** destruct (c =? c1); cbn in *.
+        reflexivity.
+        eexists; ssplit; auto.
+        econstructor; apply tr'.
+        rewrite <- EQ2; eauto.
+      * destruct e,a; cbn in *.
+        ** destruct (c =? c0); cbn in *.
            *** step in EQ1; dependent induction EQ1; inv x0.
            *** step in EQ1; inv EQ1.
-        ** destruct (c =? c1); cbn in *.
+        ** destruct (c =? c0); cbn in *.
            *** step in EQ1; dependent induction EQ1; inv x0.
            *** step in EQ1; inv EQ1.
-      * cbn in EQ1.
-        unfold Utils.mbr, MonadBr_ctree, branch in EQ1.
-        cbn in * |-.
-        rewrite unfold_bind in EQ1; cbn in EQ1.
-        inv_equ. rename EQ into eqx.
-        specialize (eqx x).
-        cbn in * |-; rewrite bind_ret_l in eqx.
-        (* setoid_rewrite <- ctree_eta in IHtr. *)
-        (* setoid_rewrite eqx in IHtr. *)
-        edestruct (IHtr (k0 x)) as (q' & comm & tr' & EQ).
-        now right; rewrite <- ctree_eta.
-        eauto.
-        exists q'; repeat split; auto.
-        eapply trans_br with (x := x).
-        eauto.
-        reflexivity.
     + inv_equ.
-  -
+      edestruct IHtr as (q' & comm & tr' & EQ).
+      left; rewrite EQ1, <- ctree_eta; reflexivity.
+      reflexivity.
+      eexists; ssplit; eauto.
+      rewrite <- EQ; now symmetry.
 
+  - destruct EQ1 as [EQ1 | EQ1]; inv_equ.
+    + unfold new in EQ1; rewrite unfold_interp in EQ1.
+      unfold trans, transR.
+      cbn.
+      desobs p; try now (step in EQ1; inv EQ1).
+      * inv_equ.
+        eexists; ssplit; auto.
+        constructor; reflexivity.
+        rewrite <- EQ2, <- ctree_eta, H; auto.
+      * destruct e,a; cbn in *.
+        ** destruct (c =? c0); cbn in *.
+           *** step in EQ1; dependent induction EQ1; inv x0.
+           *** step in EQ1; inv EQ1.
+        ** destruct (c =? c0); cbn in *.
+           *** step in EQ1; dependent induction EQ1; inv x0.
+           *** step in EQ1; inv EQ1.
 
-  - destruct EQ1 as [EQ1 | EQ1]; [ | step in EQ1; dependent induction EQ1].
+  - destruct EQ1 as [EQ1 | EQ1]; [ | inv_equ].
     unfold new in EQ1; rewrite unfold_interp in EQ1.
     unfold trans,transR; cbn.
-    desobs p; try now step in EQ1; inv EQ1.
-    + cbn in *.
-      destruct e,a; cbn in *; destruct (c =? c1) eqn:EQ; step in EQ1; dependent induction EQ1.
-    + cbn in *.
-      unfold Utils.mbr, MonadBr_ctree, branch in EQ1.
-      destruct vis; try now step in EQ1; inv EQ1.
-      rewrite unfold_bind in EQ1; cbn in EQ1.
-      inv_equ. rename EQ into eqx.
-      specialize (eqx x).
-      rewrite bind_ret_l in eqx.
-      rewrite H in eqx.
-      rewrite <- ctree_eta in EQ2.
-      rewrite EQ2 in eqx.
-      clear k t EQ2 H.
-      exists (k0 x); repeat split.
-      apply trans_brS.
-      auto.
-  - destruct EQ1 as [EQ1 | EQ1]; [ | step in EQ1; inv EQ1].
-    unfold new in EQ1; rewrite unfold_interp in EQ1.
-    unfold trans,transR; cbn.
-    desobs p; try now step in EQ1; inv EQ1.
+    desobs p; inv_equ.
     cbn in *.
-    destruct e0,a; cbn in *; destruct (c =? c0) eqn:EQ; try now step in EQ1; inv EQ1.
-    all:unfold trigger in EQ1; rewrite unfold_bind in EQ1; cbn in EQ1; setoid_rewrite bind_ret_l in EQ1.
-    all: inv_equ; rename EQ0 into eqx.
-    all:rewrite EQ.
-    all:specialize (eqx x).
-    all:rewrite H in eqx; rewrite <- ctree_eta in EQ2; rewrite EQ2 in eqx.
-    all: exists (k0 x); repeat split; auto.
-    all: apply trans_vis.
-  - tauto.
+    destruct e0,a; cbn in *; destruct (c =? c0) eqn:EQ; inv_equ.
+    + rewrite bind_trigger in EQ1.
+      inv_equ.
+      rewrite EQ; eexists; ssplit; auto.
+      constructor; reflexivity.
+      rewrite <- EQ2, <- ctree_eta, <- H; auto.
+    + rewrite bind_trigger in EQ1.
+      inv_equ.
+      rewrite EQ; eexists; ssplit; auto.
+      constructor; reflexivity.
+      rewrite <- EQ2, <- ctree_eta, <- H; auto.
+
+ - destruct EQ1 as [EQ1 | EQ1]; inv_equ.
+   unfold new in EQ1; rewrite unfold_interp in EQ1.
+   unfold trans,transR; cbn.
+   desobs p; inv_equ.
+   destruct r0.
+   cbn in *.
+   destruct e,a; cbn in *.
+   * destruct (c =? c0); cbn in *; inv_equ.
+   * destruct (c =? c0); cbn in *; inv_equ.
 Qed.
 
 Lemma trans_new_inv : forall l c p p',
@@ -534,39 +501,13 @@ Proof.
   rewrite H2, sb_guard; reflexivity.
 Qed.
 
-(** ** name restriction *)
-Lemma ctx_new_st a: unary_ctx (new a) <= st eq.
-Proof.
-  apply Coinduction, by_Symmetry. apply unary_sym.
-  intro R. apply (leq_unary_ctx (new a)). intros p q Hpq l p0 Hp0.
-  apply trans_new_inv in Hp0 as (? & comm & tr & EQ).
-  destruct (proj1 Hpq _ _ tr) as (? & ? & TR & ? & ->).
-  eapply trans_new in TR as (q' & tr' & eq'); eauto.
-  eexists; exists q'; eauto.
-  split; [|split]; eauto.
-  rewrite EQ.
-  rewrite eq'.
-  rewrite sb_guard.
-  apply unary_proper_Tctx, (id_T (sb eq)).
-  auto.
-Qed.
-
-#[global] Instance new_st a: forall R, Proper (st eq R ==> st eq R) (new a) := unary_proper_t (@ctx_new_st a).
-
 Lemma trans_plus_inv : forall l p q r,
     trans l (p + q) r ->
     (exists p', trans l p p' /\ r ≅ p') \/
       (exists q', trans l q q' /\ r ≅ q').
 Proof.
   intros * tr.
-  apply trans_brD_inv in tr as ([|] & tr); eauto.
-Qed.
-
-Lemma trans_brS' {E C X Y} : forall (c : C Y) (k : Y -> ctree E C X) x u,
-    u ≅ k x ->
-		trans tau (BrS c k) u.
-Proof.
-  intros * eq; rewrite eq; apply trans_brS.
+  apply trans_br_inv in tr as ([|] & tr); eauto.
 Qed.
 
 Lemma trans_plusL : forall l p p' q,
@@ -574,7 +515,7 @@ Lemma trans_plusL : forall l p p' q,
     trans l (p + q) p'.
 Proof.
   intros * tr.
-  now apply trans_brD21.
+  now apply trans_br21.
 Qed.
 
 Lemma trans_plusR : forall l p q q',
@@ -582,46 +523,22 @@ Lemma trans_plusR : forall l p q q',
     trans l (p + q) q'.
 Proof.
   intros * tr.
-  now apply trans_brD22.
+  now apply trans_br22.
 Qed.
-
-(** ** br *)
-Lemma ctx_plus_t: binary_ctx plus <= st eq.
-Proof.
-  apply Coinduction, by_Symmetry. apply binary_sym.
-  intro R. apply (leq_binary_ctx plus).
-  intros * [F1 B1] * [F2 B2] ? * tr.
-  apply trans_plus_inv in tr as [(? & tr & EQ) | (? & tr & EQ)].
-  - apply F1 in tr as [? (? & tr & ? & ->)].
-    do 2 eexists; split; [|split].
-    apply trans_plusL; eauto.
-    rewrite EQ.
-    now apply (id_T (sb eq)).
-    reflexivity.
-  - apply F2 in tr as [? (? & tr & ? & <-)].
-    do 2 eexists; split; [|split].
-    apply trans_plusR; eauto.
-    rewrite EQ.
-    now apply (id_T (sb eq)).
-    reflexivity.
-Qed.
-
-#[global] Instance plus_t:
-  forall R, Proper (st eq R ==> st eq R ==> st eq R) plus := binary_proper_t ctx_plus_t.
 
 Notation para_ p q :=
-  (brD3
+  (br3
      (rp <- head p;;
       match rp with
       | ARet rp => match rp with end
-      | ABr c kp => BrS c (fun i => para (kp i) q)
+      | AStep t => Step (para t q)
       | AVis e kp => Vis e (fun i => para (kp i) q)
       end)
 
      (rq <- head q;;
       match rq with
       | ARet rq => match rq with end
-      | ABr c kq => BrS c (fun i => para p (kq i))
+      | AStep t => Step (para p t)
       | AVis e kq => Vis e (fun i => para p (kq i))
       end)
 
@@ -676,13 +593,13 @@ Lemma trans_paraSynch : forall a b (p p' q q' : ccs),
     trans (comm a) p p' ->
     trans (comm b) q q' ->
     are_opposite a b ->
-    trans tau (p ∥ q) (p' ∥ q').
+    trans τ (p ∥ q) (p' ∥ q').
 Proof.
   intros * TRp TRq Op.
-  apply trans_head in TRp as (kp & TRp & Eqp).
-  apply trans_head in TRq as (kq & TRq & Eqq).
+  eapply trans_head in TRp as (kp & TRp & Eqp).
+  eapply trans_head in TRq as (kq & TRq & Eqq).
   rewrite unfold_para.
-  apply trans_brD33.
+  apply trans_br33.
   eapply trans_bind_r; [apply TRp |].
   eapply trans_bind_r; [apply TRq |].
   cbn; rewrite Op.
@@ -697,14 +614,14 @@ Lemma trans_paraL :
 Proof.
   intros * TRp.
   rewrite unfold_para.
-  apply trans_brD31.
+  apply trans_br31.
   destruct l.
-  - apply trans_head in TRp.
-    destruct TRp as (? & ? & ? & ? & TRp & Eqp).
+  - eapply trans_head in TRp.
+    destruct TRp as (? & TRp & Eqp).
     eapply trans_bind_r; eauto; cbn.
     econstructor.
     rewrite Eqp; reflexivity.
-  - apply trans_head in TRp.
+  - eapply trans_head in TRp.
     destruct TRp as (? & TRp & Eqp).
     eapply trans_bind_r; eauto; cbn.
     constructor.
@@ -719,14 +636,14 @@ Lemma trans_paraR :
 Proof.
   intros * TRq.
   rewrite unfold_para.
-  apply trans_brD32.
+  apply trans_br32.
   destruct l.
-  - apply trans_head in TRq.
-    destruct TRq as (? & ? & ? & ? & TRq & Eqq).
+  - eapply trans_head in TRq.
+    destruct TRq as (? & TRq & Eqq).
     eapply trans_bind_r; eauto; cbn.
     econstructor.
     rewrite Eqq; reflexivity.
-  - apply trans_head in TRq.
+  - eapply trans_head in TRq.
     destruct TRq as (? & TRq & Eqq).
     eapply trans_bind_r; eauto; cbn.
     constructor.
@@ -743,21 +660,21 @@ Lemma trans_para_inv :
           trans (comm a) p p' /\
             trans (comm b) q q' /\
             are_opposite a b /\
-            l = tau /\
+            l = τ /\
             r ≅ (p' ∥ q')).
 Proof.
   intros * TR.
   rewrite unfold_para in TR.
-  apply trans_brD_inv in TR as (x & TR).
+  apply trans_br_inv in TR as (x & TR).
   destruct x.
   - left.
     edestruct @trans_bind_inv; [apply TR | | ]; clear TR.
     destruct H as (NOTV & ? & TR & EQ); apply trans_head_inv in TR; easy.
     destruct H as (hdp & TRhdp & TR).
     destruct hdp; try easy.
-    * apply trans_brS_inv in TR as (x & EQ & ->).
+    * eapply trans_step_inv in TR as (EQ & ->).
       eapply trans_ABr in TRhdp.
-      eexists; split; eauto.
+      eauto.
     * apply trans_vis_inv in TR as (x & EQ & ->).
       eapply trans_AVis in TRhdp.
       eexists; split; eauto.
@@ -766,7 +683,7 @@ Proof.
     destruct H as (NOTV & ? & TR & EQ); apply trans_head_inv in TR; easy.
     destruct H as (hdq & TRhdq & TR).
     destruct hdq; try easy.
-    * apply trans_brS_inv in TR as (x & EQ & ->).
+    * apply trans_step_inv in TR as (EQ & ->).
       eapply trans_ABr in TRhdq.
       eexists; split; eauto.
     * apply trans_vis_inv in TR as (x & EQ & ->).
@@ -780,9 +697,7 @@ Proof.
     destruct H as (NOTV & ? & TR & EQ); apply trans_head_inv in TR; easy.
     destruct H as (hdq & TRhdq & TR).
     destruct hdp; try easy.
-    exfalso; eapply Stuck_is_stuck; eassumption.
     destruct hdq; try easy.
-    exfalso; eapply Stuck_is_stuck; eassumption.
     destruct e, e0, (are_opposite a a0) eqn:?.
     2:exfalso; eapply Stuck_is_stuck; eassumption.
     apply trans_step_inv in TR as [? ->].
@@ -798,187 +713,14 @@ Ltac trans_para_invT H :=
         [(?q' & ?TRq & ?EQ) |
           (?p' & ?q' & ?a & ?b & ?TRp & ?TRq & ?Op & ? & ?EQ) ]]; subst.
 
-(** ** parallel composition *)
-Lemma ctx_para_t: binary_ctx para <= st eq.
-Proof.
-  apply Coinduction, by_Symmetry. apply binary_sym.
-  intro R. apply (leq_binary_ctx para).
-  intros * [F1 B1] * [F2 B2] ? * tr.
-  trans_para_invT tr.
-  - apply F1 in TRp as [? (? & tr & ? & ?)].
-    do 2 eexists; split; [|split].
-    apply trans_paraL; eauto.
-    rewrite EQ.
-    apply (fTf_Tf (sb eq)). apply (in_binary_ctx para).
-    now apply (id_T (sb eq)).
-    now apply (b_T (sb eq)).
-    assumption.
-  - apply F2 in TRq as [? (? & tr & ? & ?)].
-    do 2 eexists; split; [|split].
-    apply trans_paraR; eauto.
-    rewrite EQ.
-    apply (fTf_Tf (sb eq)). apply (in_binary_ctx para).
-    now apply (b_T (sb eq)).
-    now apply (id_T (sb eq)).
-    assumption.
-  - apply F1 in TRp as [? (? & trp & ? & <-)].
-    apply F2 in TRq as [? (? & trq & ? & <-)].
-    do 2 eexists; split; [|split].
-    eapply trans_paraSynch; eauto.
-    rewrite EQ.
-    apply (fTf_Tf (sb eq)). apply (in_binary_ctx para); now apply (id_T (sb eq)).
-    reflexivity.
-Qed.
-
-#[global] Instance para_t: forall R, Proper (st eq R ==> st eq R ==> st eq R) para :=
-  binary_proper_t ctx_para_t.
-
-#[global] Instance para_T f: forall R, Proper (sT eq f R ==> sT eq f R ==> sT eq f R) para :=
-  binary_proper_T ctx_para_t.
-
-Section Theory.
-
-  Lemma plsC: forall (p q : ccs), p+q ~ q+p.
-  Proof.
-    apply brD2_commut.
-  Qed.
-
-  Lemma plsA (p q r : ccs): p+(q+r) ~ (p+q)+r.
-  Proof.
-    symmetry; apply brD2_assoc.
-  Qed.
-
-  Lemma pls0p (p : ccs) : 0 + p ~ p.
-  Proof.
-    apply brD2_stuckS_l.
-  Qed.
-
-  Lemma plsp0 (p : ccs) : p + 0 ~ p.
-  Proof. now rewrite plsC, pls0p. Qed.
-
-  Lemma plsidem (p : ccs) : p + p ~ p.
-  Proof.
-    apply brD2_idem.
-  Qed.
-
-  #[global] Instance are_opposite_sym : Symmetric are_opposite.
-  Proof.
-    unfold are_opposite, eqb_action, op; cbn.
-    intros [] [] Op; intuition.
-    all:rewrite eqb_sym; auto.
-  Qed.
-
-  Lemma paraC: forall (p q : ccs), p ∥ q ~ q ∥ p.
-  Proof.
-    coinduction ? CIH; symmetric using idtac.
-    intros p q l r.
-    eauto.
-    simpl.
-    intros p q ? ? tr.
-    trans_para_invT tr.
-    - do 2 eexists; split; [|split].
-      eapply trans_paraR; eauto.
-      rewrite EQ; auto.
-      reflexivity.
-    - do 2 eexists; split; [|split].
-      eapply trans_paraL; eauto.
-      rewrite EQ; auto.
-      reflexivity.
-    - do 2 eexists; split; [|split].
-      eapply trans_paraSynch; eauto.
-      symmetry; auto.
-      rewrite EQ; auto.
-      reflexivity.
-  Qed.
-
-  Lemma para0p : forall (p : ccs), 0 ∥ p ~ p.
-  Proof.
-    coinduction R CIH.
-    intros.
-    split.
-    - intros l q tr.
-      trans_para_invT tr; try now exfalso; eapply stuckS_is_stuck; eauto.
-      do 2 eexists; split; eauto.
-      rewrite EQ; auto.
-    - intros l q tr.
-      eexists.
-      exists (0 ∥ q).
-      split; eauto with trans.
-      apply trans_paraR; eauto.
-      cbn; auto.
-  Qed.
-
-  Lemma parap0 : forall (p : ccs), p ∥ 0 ~ p.
-  Proof.
-    intros; rewrite paraC; apply para0p.
-  Qed.
-
-  Lemma paraA : forall (p q r : ccs), p ∥ (q ∥ r) ~ (p ∥ q) ∥ r.
-  Proof.
-    coinduction ? CIH; intros.
-    split.
-    - intros l s tr.
-      trans_para_invT tr.
-      + do 2 eexists; split.
-        do 2 apply trans_paraL; eauto.
-        rewrite EQ; auto.
-      + trans_para_invT TRq.
-        * do 2 eexists; split.
-          apply trans_paraL, trans_paraR; eauto.
-          rewrite EQ, EQ0; auto.
-        * do 2 eexists; split.
-          apply trans_paraR; eauto.
-          rewrite EQ, EQ0; auto.
-        * do 2 eexists; split.
-          eapply trans_paraSynch; eauto.
-          eapply trans_paraR; eauto.
-          rewrite EQ, EQ0; auto.
-      + trans_para_invT TRq.
-        * do 2 eexists; split.
-          eapply trans_paraL, trans_paraSynch; eauto.
-          rewrite EQ, EQ0; auto.
-        * do 2 eexists; split.
-          eapply trans_paraSynch; eauto.
-          eapply trans_paraL; eauto.
-          rewrite EQ, EQ0; auto.
-        * inv H.
-    - intros l s tr; cbn.
-      trans_para_invT tr.
-      + trans_para_invT TRp.
-        * do 2 eexists; split.
-          apply trans_paraL; eauto.
-          rewrite EQ, EQ0; auto.
-        * do 2 eexists; split.
-          apply trans_paraR, trans_paraL; eauto.
-          rewrite EQ, EQ0; auto.
-        * do 2 eexists; split.
-          eapply trans_paraSynch; eauto.
-          eapply trans_paraL; eauto.
-          rewrite EQ, EQ0; auto.
-      + do 2 eexists; split.
-        eapply trans_paraR, trans_paraR; eauto.
-        rewrite EQ; auto.
-      + trans_para_invT TRp.
-        * do 2 eexists; split.
-          eapply trans_paraSynch; eauto.
-          eapply trans_paraR; eauto.
-          rewrite EQ, EQ0; auto.
-        * do 2 eexists; split.
-          eapply trans_paraR, trans_paraSynch; eauto.
-          rewrite EQ, EQ0; auto.
-        * inv H.
-  Qed.
-
-End Theory.
-
 Notation parabang_ p q :=
-  (brD4
+  (br4
 
      (* Communication by p *)
      (rp <- head p;;
       match rp with
       | ARet rp => match rp with end
-      | ABr c kp => BrS c (fun i => parabang (kp i) q )
+      | AStep t => Step (parabang t q)
       | AVis e kp => Vis e (fun i => parabang (kp i) q)
       end)
 
@@ -986,7 +728,7 @@ Notation parabang_ p q :=
      (rq <- head q;;
       match rq with
       | ARet rq => match rq with end
-      | ABr c kq => BrS c (fun i => (parabang (para p (kq i)) q))
+      | AStep t => Step (parabang (para p t) q)
       | AVis e kq => Vis e (fun i => (parabang (para p (kq i)) q))
       end)
 
@@ -1052,7 +794,7 @@ Proof.
     step; constructor; auto.
   - upto_bind; [apply head_equ; auto | intros hdp1 hdp2 eqp].
     inv eqp; auto.
-    step; constructor; intros ?.
+    step; constructor.
     apply CIH; auto; rewrite EQp, H; reflexivity.
     step; constructor; intros ?.
     apply CIH; auto; rewrite EQp, H; reflexivity.
@@ -1061,7 +803,7 @@ Proof.
     inv eqp; auto.
     inv eqq; auto.
     destruct e, e0, (are_opposite a a0); auto.
-    step; constructor; intros ?.
+    step; constructor.
     apply CIH; auto.
     rewrite H,H0; reflexivity.
   - upto_bind; [apply head_equ; auto | intros hdp1 hdp2 eqp].
@@ -1069,7 +811,7 @@ Proof.
     inv eqp; auto.
     inv eqq; auto.
     destruct e, e0, (are_opposite a a0); auto.
-    step; constructor; intros ?.
+    step; constructor.
     apply CIH; auto.
     rewrite EQp, H,H0; reflexivity.
 Qed.
@@ -1079,9 +821,9 @@ Lemma trans_parabangL : forall p l p' q,
     trans l (parabang p q) (parabang p' q).
 Proof.
   intros * TR.
-  pose proof trans_head TR.
+  epose proof trans_head TR.
   rewrite unfold_parabang.
-  apply trans_brD41.
+  apply trans_br41.
   destruct l;
     repeat match goal with
            | h : Logic.ex _ |- _ => destruct h
@@ -1099,9 +841,9 @@ Lemma trans_parabangR : forall p l q q',
     trans l (parabang p q) (parabang (p ∥ q') q).
 Proof.
   intros * TR.
-  pose proof trans_head TR.
+  epose proof trans_head TR.
   rewrite unfold_parabang.
-  apply trans_brD42.
+  apply trans_br42.
   destruct l;
     repeat match goal with
            | h : Logic.ex _ |- _ => destruct h
@@ -1118,13 +860,13 @@ Lemma trans_parabangSL : forall a b p p' q q',
     are_opposite a b ->
     trans (comm a) p p' ->
     trans (comm b) q q' ->
-    trans tau (parabang p q) (parabang (p' ∥ q') q).
+    trans τ (parabang p q) (parabang (p' ∥ q') q).
 Proof.
   intros * Op TR1 TR2.
-  pose proof trans_head TR1 as (? & TRh1 & EQ1).
-  pose proof trans_head TR2 as (? & TRh2 & EQ2).
+  epose proof trans_head TR1 as (? & TRh1 & EQ1).
+  epose proof trans_head TR2 as (? & TRh2 & EQ2).
   rewrite unfold_parabang.
-  apply trans_brD43.
+  apply trans_br43.
   eapply trans_bind_r; [apply TRh1 | ].
   eapply trans_bind_r; [apply TRh2 | ].
   cbn; rewrite Op.
@@ -1136,13 +878,13 @@ Lemma trans_parabangSR : forall a b p q q' q'',
     are_opposite a b ->
     trans (comm a) q q' ->
     trans (comm b) q q'' ->
-    trans tau (parabang p q) (parabang (p ∥ (q' ∥ q'')) q).
+    trans τ (parabang p q) (parabang (p ∥ (q' ∥ q'')) q).
 Proof.
   intros * Op TR1 TR2.
-  pose proof trans_head TR1 as (? & TRh1 & EQ1).
-  pose proof trans_head TR2 as (? & TRh2 & EQ2).
+  epose proof trans_head TR1 as (? & TRh1 & EQ1).
+  epose proof trans_head TR2 as (? & TRh2 & EQ2).
   rewrite unfold_parabang.
-  apply trans_brD44.
+  apply trans_br44.
   eapply trans_bind_r; [apply TRh1 | ].
   eapply trans_bind_r; [apply TRh2 | ].
   cbn; rewrite Op.
@@ -1157,23 +899,23 @@ Lemma trans_parabang_inv : forall l p q r,
       (exists a b p' q', trans (comm a) p p' /\
                       trans (comm b) q q' /\
                       are_opposite a b /\
-                      l = tau /\
+                      l = τ /\
                       r ≅ parabang (p' ∥ q') q) \/
       (exists a b q' q'', trans (comm a) q q' /\
                        trans (comm b) q q'' /\
                        are_opposite a b /\
-                       l = tau /\
+                       l = τ /\
                        r ≅ parabang (p ∥ (q' ∥ q'')) q).
 Proof.
   intros * TR.
   rewrite unfold_parabang in TR.
-  apply trans_brD_inv in TR as [[]  TR].
+  apply trans_br_inv in TR as [[]  TR].
   - left.
     apply trans_bind_inv in TR.
     destruct TR as [(NV & ? & TR & ?) | (? & TR1 & TR2)]; [apply trans_head_inv in TR; easy|].
     destruct x; try easy.
-    apply trans_brS_inv in TR2 as (x & EQ & ->).
-    pose proof trans_ABr TR1 x.
+    apply trans_step_inv in TR2 as (EQ & ->).
+    pose proof trans_ABr TR1.
     eauto.
     apply trans_vis_inv in TR2 as (x & EQ & ->).
     pose proof trans_AVis TR1 (i := x).
@@ -1182,8 +924,8 @@ Proof.
     apply trans_bind_inv in TR.
     destruct TR as [(NV & ? & TR & ?) | (? & TR1 & TR2)]; [apply trans_head_inv in TR; easy|].
     destruct x; try easy.
-    apply trans_brS_inv in TR2 as (x & EQ & ->).
-    pose proof trans_ABr TR1 x.
+    apply trans_step_inv in TR2 as (EQ & ->).
+    pose proof trans_ABr TR1.
     eauto.
     apply trans_vis_inv in TR2 as (x & EQ & ->).
     pose proof trans_AVis TR1 (i := x).
@@ -1229,10 +971,232 @@ Ltac pL := apply trans_paraL.
 Ltac pR := apply trans_paraR.
 Ltac pS := eapply trans_paraSynch.
 
+Ltac inv_ccs_trans :=
+  match goal with
+  | h : hrel_of (trans _) (prefix _ _) _ |- _ => apply trans_prefix_inv in h as (?EQ & ->)
+  | h : hrel_of (trans _) (new _ _) _ |- _ => apply trans_new_inv in h as (?q & ?EQ & ?tr & ?EQ')
+  | h : hrel_of (trans _) (plus _ _) _ |- _ => apply trans_plus_inv in h as [(?q & ?tr & ?EQ) | (?q & ?tr & ?EQ)]
+  | h : hrel_of (trans _) (para _ _) _ |- _ => trans_para_invT h
+  | h : hrel_of (trans _) (parabang _ _) _ |- _ => trans_parabang_invT h
+  | h : hrel_of (trans _) (bang _) _ |- _ => trans_parabang_invT h
+  | _ => idtac
+  end.
+Hint Resolve trans_prefix trans_new trans_plusL trans_plusR trans_paraSynch trans_paraL trans_paraR
+             trans_parabangL trans_parabangR trans_parabangSL trans_parabangSR
+  : ccs.
+Ltac ccs_trans := eauto with ccs.
+
+(** ** prefix  *)
+#[global] Instance prefix_st a: forall (R : Chain (sb eq)),
+    Proper (elem R ==> elem R) (prefix a).
+Proof.
+  apply (Proper_symchain 1).
+  intros R HR p q Hpq l p' pp'.
+  inv_ccs_trans.
+  eex; ssplit; ccs_trans.
+  rewrite EQ.
+  now step.
+Qed.
+
+(** ** name restriction *)
+#[global] Instance ctx_new_st c: forall (R : Chain (sb eq)),
+    Proper (elem R ==> elem R) (new c).
+Proof.
+  cbn.
+  apply (Proper_symchain 1).
+  intros R HR p q Hpq l p' pp'.
+  inv_ccs_trans.
+  apply Hpq in tr as (? & ? & ? & ? & ?); subst.
+  eapply trans_new in EQ as (? & ? & ?); eauto.
+  eex; ssplit; ccs_trans.
+  rewrite H2, EQ'.
+  rewrite sb_guard.
+  now apply HR.
+Qed.
+
+(** ** plus  *)
+#[global] Instance ctx_plus_t : forall (R : Chain (sb eq)),
+  Proper (elem R ==> elem R ==> elem R) plus.
+Proof.
+  cbn.
+  apply (Proper_symchain 2).
+  intros R HR p q Hpq r s Hrs l p' pp'.
+  inv_ccs_trans.
+  - apply Hpq in tr as (? & ? & ? & ? & ?); subst.
+    eex; ssplit; ccs_trans.
+    now rewrite EQ.
+  - apply Hrs in tr as (? & ? & ? & ? & ?); subst.
+    eex; ssplit; ccs_trans.
+    now rewrite EQ.
+Qed.
+
+(** ** parallel composition *)
+#[global] Instance ctx_para_t: forall (R : Chain (sb eq)),
+  Proper (elem R ==> elem R ==> elem R) para.
+Proof.
+  cbn.
+  apply (Proper_symchain 2).
+  intros R HR p q FB1 r s FB2 l p' pp'.
+  inv_ccs_trans.
+  - apply FB1 in TRp as [? (? & tr & ? & ?)].
+    do 2 eexists; split; [|split].
+    apply trans_paraL; eauto.
+    rewrite EQ.
+    apply HR; auto.
+    2:auto.
+    step; apply FB2.
+  - apply FB2 in TRq as [? (? & tr & ? & ?)].
+    do 2 eexists; split; [|split].
+    apply trans_paraR; eauto.
+    rewrite EQ.
+    2:auto.
+    apply HR; auto.
+    step; auto.
+  - apply FB1 in TRp as [? (? & trp & ? & <-)].
+    apply FB2 in TRq as [? (? & trq & ? & <-)].
+    do 2 eexists; split; [|split].
+    eapply trans_paraSynch; eauto.
+    rewrite EQ.
+    apply HR; auto.
+    auto.
+Qed.
+
+Section Theory.
+
+  Lemma plsC: forall (p q : ccs), p+q ~ q+p.
+  Proof.
+    apply br2_commut.
+  Qed.
+
+  Lemma plsA (p q r : ccs): p+(q+r) ~ (p+q)+r.
+  Proof.
+    symmetry; apply br2_assoc.
+  Qed.
+
+  Lemma pls0p (p : ccs) : 0 + p ~ p.
+  Proof.
+    apply br2_stuck_l.
+  Qed.
+
+  Lemma plsp0 (p : ccs) : p + 0 ~ p.
+  Proof. now rewrite plsC, pls0p. Qed.
+
+  Lemma plsidem (p : ccs) : p + p ~ p.
+  Proof.
+    apply br2_idem.
+  Qed.
+
+  #[global] Instance are_opposite_sym : Symmetric are_opposite.
+  Proof.
+    unfold are_opposite, eqb_action, op; cbn.
+    intros [] [] Op; intuition.
+    all:rewrite eqb_sym; auto.
+  Qed.
+
+  Lemma paraC: forall (p q : ccs), p ∥ q ~ q ∥ p.
+  Proof.
+    coinduction r CIH; symmetric.
+    intros p q ? ? tr.
+    trans_para_invT tr.
+    - do 2 eexists; split; [|split].
+      eapply trans_paraR; eauto.
+      rewrite EQ; auto.
+      reflexivity.
+    - do 2 eexists; split; [|split].
+      eapply trans_paraL; eauto.
+      rewrite EQ; auto.
+      reflexivity.
+    - do 2 eexists; split; [|split].
+      eapply trans_paraSynch; eauto.
+      symmetry; auto.
+      rewrite EQ; auto.
+      reflexivity.
+  Qed.
+
+  Lemma para0p : forall (p : ccs), 0 ∥ p ~ p.
+  Proof.
+    coinduction R CIH.
+    intros.
+    split.
+    - intros l q tr.
+      trans_para_invT tr; try now exfalso; eapply Stuck_is_stuck; eauto.
+      do 2 eexists; split; eauto.
+      rewrite EQ; auto.
+    - intros l q tr.
+      eexists.
+      exists (0 ∥ q).
+      split; eauto with trans.
+      apply trans_paraR; eauto.
+      cbn; auto.
+  Qed.
+
+  Lemma parap0 : forall (p : ccs), p ∥ 0 ~ p.
+  Proof.
+    intros; rewrite paraC; apply para0p.
+  Qed.
+
+  Lemma paraA : forall (p q r : ccs), p ∥ (q ∥ r) ~ (p ∥ q) ∥ r.
+  Proof.
+    coinduction r CIH; intros.
+    split.
+    - intros l s tr.
+      trans_para_invT tr.
+      + do 2 eexists; split.
+        do 2 apply trans_paraL; eauto.
+        rewrite EQ; auto.
+      + trans_para_invT TRq.
+        * do 2 eexists; split.
+          apply trans_paraL, trans_paraR; eauto.
+          rewrite EQ, EQ0; auto.
+        * do 2 eexists; split.
+          apply trans_paraR; eauto.
+          rewrite EQ, EQ0; auto.
+        * do 2 eexists; split.
+          eapply trans_paraSynch; eauto.
+          eapply trans_paraR; eauto.
+          rewrite EQ, EQ0; auto.
+      + trans_para_invT TRq.
+        * do 2 eexists; split.
+          eapply trans_paraL, trans_paraSynch; eauto.
+          rewrite EQ, EQ0; auto.
+        * do 2 eexists; split.
+          eapply trans_paraSynch; eauto.
+          eapply trans_paraL; eauto.
+          rewrite EQ, EQ0; auto.
+        * inv H.
+    - intros l s tr; cbn.
+      trans_para_invT tr.
+      + trans_para_invT TRp.
+        * do 2 eexists; split.
+          apply trans_paraL; eauto.
+          rewrite EQ, EQ0; auto.
+        * do 2 eexists; split.
+          apply trans_paraR, trans_paraL; eauto.
+          rewrite EQ, EQ0; auto.
+        * do 2 eexists; split.
+          eapply trans_paraSynch; eauto.
+          eapply trans_paraL; eauto.
+          rewrite EQ, EQ0; auto.
+      + do 2 eexists; split.
+        eapply trans_paraR, trans_paraR; eauto.
+        rewrite EQ; auto.
+      + trans_para_invT TRp.
+        * do 2 eexists; split.
+          eapply trans_paraSynch; eauto.
+          eapply trans_paraR; eauto.
+          rewrite EQ, EQ0; auto.
+        * do 2 eexists; split.
+          eapply trans_paraR, trans_paraSynch; eauto.
+          rewrite EQ, EQ0; auto.
+        * inv H.
+  Qed.
+
+End Theory.
+
 Lemma para_parabang : forall p q r,
     parabang (p ∥ q) r ~ p ∥ parabang q r.
 Proof.
-  coinduction ? CIH.
+  coinduction R CIH.
   intros; split.
   - intros l s TR.
     trans_parabang_invT TR.
@@ -1247,18 +1211,20 @@ Proof.
         pS; eauto.
         pbL; eauto.
         rewrite EQ,EQ0; auto.
-    + do 2 eexists; split.
+    + do 2 eexists; ssplit.
       pR; pbR; eauto.
-      rewrite EQ, !CIH, paraA; auto.
-
+      2:auto.
+      now rewrite EQ, 2CIH, paraA.
     + trans_para_invT TRp'.
-      * do 2 eexists; split.
+      * eex; ssplit.
         pS; eauto.
         pbR; eauto.
-        rewrite EQ,EQ0, !CIH, !paraA; eauto.
-      * do 2 eexists; split.
+        2:auto.
+        now rewrite EQ,EQ0,2CIH, paraA.
+      * eex; ssplit.
         pR; pbSL; eauto.
-        rewrite EQ,EQ0, !CIH, !paraA; eauto.
+        2:auto.
+        now rewrite EQ,EQ0,2CIH, paraA.
       * easy.
 
     + do 2 eexists; split.
@@ -1298,65 +1264,55 @@ Proof.
       * easy.
 Qed.
 
-Lemma ctx_parabang_t: binary_ctx parabang <= st eq.
+#[global] Instance ctx_parabang_t: forall (R : Chain (sb eq)),
+    Proper (elem R ==> elem R ==> elem R) parabang.
 Proof.
-  apply Coinduction, by_Symmetry. apply binary_sym.
-  intro R. apply (leq_binary_ctx parabang).
-  intros * [F1 B1] * [F2 B2] ? * tr.
-  trans_parabang_invT tr.
-  - apply F1 in TRp' as [? (? & tr & ? & ?)].
-    do 2 eexists; split; [|split].
+  cbn.
+  apply (Proper_symchain 2).
+  intros R HR p q FB1 r s FB2 l p' pp'.
+  inv_ccs_trans.
+  - apply FB1 in TRp' as [? (? & tr & ? & ?)].
+    eex; ssplit.
     pbL; eauto.
     rewrite EQ.
-    apply (fTf_Tf (sb eq)). apply (in_binary_ctx parabang).
-    now apply (id_T (sb eq)).
-    now apply (b_T (sb eq)).
+    apply HR; auto.
+    step; auto.
     assumption.
-  - apply F2 in TRq' as [? (? & tr & ? & ?)].
-    do 2 eexists; split; [|split].
+  - apply FB2 in TRq' as [? (? & tr & ? & ?)].
+    eex; ssplit.
     pbR; eauto.
     rewrite EQ.
-    apply (fTf_Tf (sb eq)). apply (in_binary_ctx parabang).
-    apply (fT_T ctx_para_t).
-    apply (in_binary_ctx para).
-    now apply (b_T (sb eq)).
-    now apply (id_T (sb eq)).
-    now apply (b_T (sb eq)).
+    apply HR; auto.
+    apply ctx_para_t; auto.
+    step; auto.
+    step; auto.
     assumption.
-  - apply F1 in TRp' as [? (? & trp & ? & <-)].
-    apply F2 in TRq' as [? (? & trq & ? & <-)].
-    do 2 eexists; split; [|split].
+  - apply FB1 in TRp' as [? (? & trp & ? & <-)].
+    apply FB2 in TRq' as [? (? & trq & ? & <-)].
+    eex; ssplit.
     pbSL; eauto.
     rewrite EQ.
-    apply (fTf_Tf (sb eq)). apply (in_binary_ctx parabang).
-    apply (fT_T ctx_para_t).
-    apply (in_binary_ctx para).
-    now apply (id_T (sb eq)).
-    now apply (id_T (sb eq)).
-    now apply (b_T (sb eq)).
-    reflexivity.
-  - apply F2 in TRq' as  [? (? & trq' & ? & <-)].
-    apply F2 in TRq'' as  [? (? & trq'' & ? & <-)].
-    do 2 eexists; split; [|split].
+    apply HR; auto.
+    apply ctx_para_t; auto.
+    step; auto.
+    auto.
+  - apply FB2 in TRq' as  [? (? & trq' & ? & <-)].
+    apply FB2 in TRq'' as  [? (? & trq'' & ? & <-)].
+    eex; ssplit.
     pbSR; eauto.
     rewrite EQ.
-    apply (fTf_Tf (sb eq)). apply (in_binary_ctx parabang).
-    apply (fT_T ctx_para_t), (in_binary_ctx para).
-    now apply (b_T (sb eq)).
-    apply (fT_T ctx_para_t), (in_binary_ctx para).
-    now apply (id_T (sb eq)).
-    now apply (id_T (sb eq)).
-    now apply (b_T (sb eq)).
-    reflexivity.
+    apply HR; auto.
+    apply ctx_para_t; auto.
+    step; auto.
+    apply ctx_para_t; auto.
+    step; auto.
+    auto.
 Qed.
-
-#[global] Instance parabang_t: forall R, Proper (st eq R ==> st eq R ==> st eq R) parabang := binary_proper_t ctx_parabang_t.
-#[global] Instance parabang_T f: forall R, Proper (sT eq f R ==> sT eq f R ==> sT eq f R) parabang := binary_proper_T ctx_parabang_t.
 
 Lemma parabang_aux : forall p q,
     parabang (p ∥ q) q ~ parabang p q.
 Proof.
-  coinduction ? CIH.
+  coinduction R CIH.
   split.
   - intros l r TR.
     trans_parabang_invT TR.
@@ -1427,7 +1383,7 @@ Qed.
 Lemma parabang_eq : forall p q,
     parabang p q ~ p ∥ !q.
 Proof.
-  coinduction ? CIH.
+  coinduction R CIH.
   intros p q; split.
 
   - intros l p' TR.
